Refinement of interleaving fold. Also avoid copying when coparing shared variables

PAC_Checker_LLVM/Interleaving_Fold.thy
@@ -1,5 +1,5 @@
 theory Interleaving_Fold
-  imports Main
+  imports IICF_Copying_List
 begin
 
 text \<open>This theory defines a generalization of the
@@ -26,5 +26,754 @@ fun ifoldl :: \<open>('a \<Rightarrow> 'b \<Rightarrow> 'c \<Rightarrow> directi
     | RIGHT \<Rightarrow> ifoldl f dec f1 f2 (f acc x y RIGHT) (x # xs) ys
     | BOTH  \<Rightarrow> ifoldl f dec f1 f2 (f acc x y BOTH)  xs ys
   )\<close>
+
+definition foldl_nres :: \<open>('a \<Rightarrow> 'b \<Rightarrow> 'a nres) \<Rightarrow> 'a \<Rightarrow> 'b list \<Rightarrow> 'a nres\<close> where
+  \<open>foldl_nres f acc xs \<equiv> REC\<^sub>T (\<lambda>fr (acc, xs). doN {
+    if xs = [] then RETURN acc 
+    else doN {
+      (x,xs) \<leftarrow> mop_list_pop_hd xs;
+      acc \<leftarrow> f acc x;
+      fr (acc, xs) 
+    } 
+  }) (acc, xs)\<close>
+
+definition ifoldl_nres :: \<open>('a \<Rightarrow> 'b \<Rightarrow> 'c \<Rightarrow> direction \<Rightarrow> 'a nres) \<Rightarrow> ('b \<Rightarrow> 'c \<Rightarrow> direction nres)
+  \<Rightarrow> ('a \<Rightarrow> 'b \<Rightarrow> 'a nres) \<Rightarrow> ('a \<Rightarrow> 'c \<Rightarrow> 'a nres)
+  \<Rightarrow> 'a \<Rightarrow> 'b list \<Rightarrow> 'c list \<Rightarrow> 'a nres\<close> where
+  \<open>ifoldl_nres f dec f1 f2 acc xs ys \<equiv> doN {
+    (acc, xs, ys, stop) \<leftarrow> WHILEIT
+      (\<lambda>_. True)
+      (\<lambda>(acc, xs, ys, stop). xs \<noteq> [] \<and> ys \<noteq> [] \<and> \<not>stop)
+      (\<lambda>(acc, xs, ys, stop). doN {
+        ASSERT (xs \<noteq> [] \<and> ys \<noteq> []);
+        (x,xs) \<leftarrow> mop_list_pop_hd xs;
+        (y,ys) \<leftarrow> mop_list_pop_hd ys;
+        dir \<leftarrow> dec x y;
+        acc \<leftarrow> f acc x y dir;
+        if dir = STOP then RETURN (acc, xs, ys, True)
+        else if dir = LEFT then RETURN (acc, xs, y # ys, False)
+        else if dir = RIGHT then RETURN (acc, x # xs, ys, False)
+        else RETURN (acc, xs, ys, False)
+      })
+      (acc, xs, ys, False);
+    if stop then RETURN acc
+    else if ys = [] then foldl_nres f1 acc xs
+    else if xs = [] then foldl_nres f2 acc ys
+    else RETURN acc
+  }\<close>
+
+lemma WHILEIT_true_rule:
+  assumes WF: \<open>wf R\<close>
+    and I0: \<open>I s\<close>
+    and IS: \<open>\<And>s. \<lbrakk>I s; b s\<rbrakk> \<Longrightarrow> f s \<le> SPEC (\<lambda>s'. I s' \<and> (s', s) \<in> R)\<close>
+    and PHI: \<open>\<And>s. \<lbrakk>I s; \<not>b s\<rbrakk> \<Longrightarrow> \<Phi> s\<close>
+  shows \<open>WHILEIT (\<lambda>_. True) b f s \<le> SPEC \<Phi>\<close>
+  using WHILET_rule[OF assms] unfolding WHILET_def .
+
+lemma foldl_nres_unfold:
+  \<open>foldl_nres f acc xs = doN {
+    if xs = [] then RETURN acc
+    else doN {
+      (x, xs) \<leftarrow> mop_list_pop_hd xs;
+      acc \<leftarrow> f acc x;
+      foldl_nres f acc xs
+    }
+  }\<close>
+  unfolding foldl_nres_def
+  apply (subst RECT_unfold)
+  subgoal by refine_mono
+  subgoal by simp
+  done
+
+lemma foldl_nres_refine:
+  assumes f: \<open>\<And>acc x. fn acc x \<le> SPEC (\<lambda>r. r = f acc x)\<close>
+  shows \<open>foldl_nres fn acc xs \<le> SPEC (\<lambda>r. r = foldl f acc xs)\<close>
+proof (induction xs arbitrary: acc)
+  case Nil
+  show ?case by (subst foldl_nres_unfold) simp
+next
+  case (Cons x xs acc)
+  show ?case
+    apply (subst foldl_nres_unfold)
+    apply (use Cons.IH[of \<open>f acc x\<close>] f[of acc x] in
+        \<open>auto simp: pw_le_iff refine_pw_simps mop_list_pop_hd_def\<close>)
+    done
+qed
+
+lemma ifoldl_Nil2: \<open>ifoldl f dec f1 f2 acc xs [] = foldl f1 acc xs\<close>
+  by (cases xs) auto
+
+lemma ifoldl_Nil1: \<open>ifoldl f dec f1 f2 acc [] ys = foldl f2 acc ys\<close>
+  by (cases ys) auto
+
+lemma ifoldl_nres_refine:
+  assumes f: \<open>\<And>acc x y dir. fn acc x y dir \<le> SPEC (\<lambda>r. r = f acc x y dir)\<close>
+      and dec: \<open>\<And>x y. decn x y \<le> SPEC (\<lambda>r. r = dec x y)\<close>
+      and f1: \<open>\<And>acc x. f1n acc x \<le> SPEC (\<lambda>r. r = f1 acc x)\<close>
+      and f2: \<open>\<And>acc y. f2n acc y \<le> SPEC (\<lambda>r. r = f2 acc y)\<close>
+    shows \<open>ifoldl_nres fn decn f1n f2n acc xs ys \<le> SPEC (\<lambda>r. r = ifoldl f dec f1 f2 acc xs ys)\<close>
+  unfolding ifoldl_nres_def
+  apply (rule bind_rule)
+  apply (rule WHILEIT_true_rule[where
+        I = \<open>\<lambda>(acc', xs', ys', stop).
+              (if stop then acc' else ifoldl f dec f1 f2 acc' xs' ys')
+                = ifoldl f dec f1 f2 acc xs ys\<close>
+        and R = \<open>measure (\<lambda>(acc', xs', ys', stop).
+              (if stop then 0 else length xs' + length ys' + 1))\<close>])
+  subgoal by simp
+  subgoal by simp
+  subgoal for s
+    apply (cases s rule: prod_cases4)
+    apply (simp only: prod.case)
+    apply (elim conjE)
+    apply (cases \<open>fst (snd s)\<close>; cases \<open>fst (snd (snd s))\<close>)
+    apply (simp_all add: mop_list_pop_hd_def)
+    apply (rule bind_rule)
+    apply (rule order_trans[OF dec])
+    apply (rule SPEC_rule)
+    apply (rule bind_rule)
+    apply (rule order_trans[OF f])
+    apply (rule SPEC_rule)
+    apply (auto split: direction.splits)
+    done
+  subgoal for s
+    apply (cases s rule: prod_cases4)
+    apply (auto simp: ifoldl_Nil1 ifoldl_Nil2
+        intro: order_trans[OF foldl_nres_refine[OF f1]]
+               order_trans[OF foldl_nres_refine[OF f2]])
+    done
+  done
+
+subsection \<open>Unfolding equations for @{term ifoldl_nres}\<close>
+
+lemma foldl_nres_Nil[simp]: \<open>foldl_nres f acc [] = RETURN acc\<close>
+  by (subst foldl_nres_unfold) simp
+
+lemma foldl_nres_Cons:
+  \<open>foldl_nres f acc (x # xs) = doN {acc \<leftarrow> f acc x; foldl_nres f acc xs}\<close>
+  by (subst foldl_nres_unfold) (simp add: mop_list_pop_hd_def)
+
+lemma ifoldl_nres_Nil2: \<open>ifoldl_nres fn decn f1n f2n acc xs [] = foldl_nres f1n acc xs\<close>
+  unfolding ifoldl_nres_def by (subst WHILEIT_unfold) simp
+
+lemma ifoldl_nres_Nil1: \<open>ifoldl_nres fn decn f1n f2n acc [] ys = foldl_nres f2n acc ys\<close>
+  unfolding ifoldl_nres_def by (subst WHILEIT_unfold) (cases ys; simp)
+
+lemma ifoldl_nres_Cons:
+  \<open>ifoldl_nres fn decn f1n f2n acc (x # xs) (y # ys) = doN {
+    dir \<leftarrow> decn x y;
+    acc \<leftarrow> fn acc x y dir;
+    case dir of
+      STOP \<Rightarrow> RETURN acc
+    | LEFT \<Rightarrow> ifoldl_nres fn decn f1n f2n acc xs (y # ys)
+    | RIGHT \<Rightarrow> ifoldl_nres fn decn f1n f2n acc (x # xs) ys
+    | BOTH \<Rightarrow> ifoldl_nres fn decn f1n f2n acc xs ys
+  }\<close>
+  unfolding ifoldl_nres_def
+  apply (subst WHILEIT_unfold)
+  apply (simp add: mop_list_pop_hd_def)
+  apply (intro bind_cong[OF refl] ext)
+  apply (auto split: direction.splits)
+  text \<open>Remaining: the \<open>STOP\<close> case, where the loop exits at once.\<close>
+  apply (subst WHILEIT_unfold)
+  apply simp
+  done
+
+section \<open>Implementation for Copying Lists\<close>
+
+definition[llvm_code]: \<open>cl_foldl_monadic' f \<equiv> MMonad.REC (\<lambda>ff (acc, p).
+  if p = null then Mreturn acc
+  else doM {
+    n \<leftarrow> ll_load p;
+    acc \<leftarrow> f acc (node.val n);
+    ff (acc, node.next n)
+  })\<close>
+
+lemmas cl_foldl_monadic'_unfold = REC_unfold_extr[OF cl_foldl_monadic'_def, discharge_monos]
+
+lemma cl_fold_monadic'_rule:
+  assumes F: \<open>\<And>a ai b bi. llvm_htriple (A a ai ** B b bi) (fi ai bi) (\<lambda>r. A (f a b) r ** B b bi)\<close>
+  shows \<open>llvm_htriple
+    (A a ai ** cl_assn' B bs bsi)
+    (cl_foldl_monadic' fi (ai, bsi))
+    (\<lambda>r. A (foldl f a bs) r ** cl_assn' B bs bsi)\<close>
+proof (induction bs arbitrary: a ai bsi)
+  case Nil
+  show ?case
+    supply [simp] = cl_assn_simps
+    apply (subst cl_foldl_monadic'_unfold)
+    by vcg
+next
+  case (Cons b bs)
+  note [vcg_rules] = Cons.IH F
+  show ?case
+    supply [simp] = cl_assn_simps
+    apply (subst cl_foldl_monadic'_unfold)
+    by vcg
+qed
+
+lemma cl_fold_hfref:
+  assumes F: \<open>(uncurry fi, uncurry (RETURN oo f)) \<in> A\<^sup>d *\<^sub>a B\<^sup>k \<rightarrow>\<^sub>a A\<close>
+  shows \<open>(cl_foldl_monadic' fi, uncurry (RETURN oo foldl f))
+        \<in> A\<^sup>d *\<^sub>a (cl_assn' B)\<^sup>k \<rightarrow>\<^sub>a A\<close>
+proof -
+  have BODY: \<open>llvm_htriple (A a ai ** B b bi) (fi ai bi)
+                (\<lambda>r. A (f a b) r ** B b bi)\<close> for a ai b bi
+    apply (rule htriple_ent_post[OF _ hfref_htriple_d1_k2[OF F]])
+    by (simp add: sep_conj_aci)
+  show ?thesis
+    supply [vcg_rules] = cl_fold_monadic'_rule[where A=A and B=B and fi=fi and f=f, OF BODY]
+    by (sepref_to_hoare; vcg)
+qed
+
+text \<open>Refinement of the monadic fold @{term foldl_nres}: the step function is an
+  \<open>nres\<close> program, so its rule carries a \<open>nofail\<close> premise and a refinement
+  postcondition (the shape of @{thm hn_refineD}).\<close>
+lemma cl_fold_monadic'_nres_rule:
+  assumes F: \<open>\<And>a ai b bi. nofail (f a b) \<Longrightarrow> llvm_htriple
+    (A a ai ** B b bi) (fi ai bi)
+    (\<lambda>r. B b bi ** (EXS x. A x r ** \<up>(RETURN x \<le> f a b)))\<close>
+  assumes NF: \<open>nofail (foldl_nres f a bs)\<close>
+  shows \<open>llvm_htriple
+    (A a ai ** cl_assn' B bs bsi)
+    (cl_foldl_monadic' fi (ai, bsi))
+    (\<lambda>r. cl_assn' B bs bsi ** (EXS x. A x r ** \<up>(RETURN x \<le> foldl_nres f a bs)))\<close>
+  using NF
+proof (induction bs arbitrary: a ai bsi)
+  case Nil
+  show ?case
+    supply [simp] = cl_assn_simps
+    apply (subst cl_foldl_monadic'_unfold)
+    apply (subst foldl_nres_unfold)
+    by vcg
+next
+  case (Cons b bs)
+  note [vcg_rules] = F Cons.IH
+  show ?case
+    using Cons.prems
+    supply [simp] = cl_assn_simps refine_pw_simps pw_le_iff mop_list_pop_hd_def
+    apply (subst (asm) foldl_nres_unfold)
+    apply (subst cl_foldl_monadic'_unfold)
+    apply (subst foldl_nres_unfold)
+    by vcg
+qed
+
+text \<open>Variant with the \<open>nofail\<close> condition in the precondition. As a rule premise
+  it is checked before the pure parts of the current state are extracted, which
+  loses facts such as \<open>drop j cs = []\<close> obtained from \<open>cl_assn' C (drop j cs) null\<close>.\<close>
+lemma cl_fold_monadic'_nres_rule':
+  assumes F: \<open>\<And>a ai b bi. nofail (f a b) \<Longrightarrow> llvm_htriple
+    (A a ai ** B b bi) (fi ai bi)
+    (\<lambda>r. B b bi ** (EXS x. A x r ** \<up>(RETURN x \<le> f a b)))\<close>
+  shows \<open>llvm_htriple
+    (A a ai ** cl_assn' B bs bsi ** \<up>(nofail (foldl_nres f a bs)))
+    (cl_foldl_monadic' fi (ai, bsi))
+    (\<lambda>r. cl_assn' B bs bsi ** (EXS x. A x r ** \<up>(RETURN x \<le> foldl_nres f a bs)))\<close>
+proof (rule htriple_pure_preI)
+  assume \<open>pure_part (A a ai ** cl_assn' B bs bsi ** \<up>(nofail (foldl_nres f a bs)))\<close>
+  then have NF: \<open>nofail (foldl_nres f a bs)\<close>
+    by (auto dest!: pure_part_split_conj)
+  show \<open>llvm_htriple
+    (A a ai ** cl_assn' B bs bsi ** \<up>(nofail (foldl_nres f a bs)))
+    (cl_foldl_monadic' fi (ai, bsi))
+    (\<lambda>r. cl_assn' B bs bsi ** (EXS x. A x r ** \<up>(RETURN x \<le> foldl_nres f a bs)))\<close>
+    apply (rule htriple_ent_pre[OF _ cl_fold_monadic'_nres_rule[OF F NF]])
+    by (auto simp: entails_def sep_algebra_simps pred_lift_extract_simps)
+qed
+
+lemma cl_fold_monadic'_hfref:
+  assumes F: \<open>(uncurry fi, uncurry f) \<in> A\<^sup>d *\<^sub>a B\<^sup>k \<rightarrow>\<^sub>a A\<close>
+  shows \<open>(cl_foldl_monadic' fi, uncurry (foldl_nres f))
+        \<in> A\<^sup>d *\<^sub>a (cl_assn' B)\<^sup>k \<rightarrow>\<^sub>a A\<close>
+proof -
+  note HT = F[to_hnr, unfolded autoref_tag_defs, THEN hn_refineD]
+  have BODY: \<open>llvm_htriple (A a ai ** B b bi) (fi ai bi)
+      (\<lambda>r. B b bi ** (EXS x. A x r ** \<up>(RETURN x \<le> f a b)))\<close>
+    if NF: \<open>nofail (f a b)\<close> for a ai b bi
+    apply (rule htriple_ent_pre[OF _ htriple_ent_post[OF _ HT[OF NF]]])
+    unfolding hn_ctxt_def
+    subgoal by (rule entails_refl)
+    subgoal
+      by (auto simp: entails_def sep_algebra_simps sep_conj_exists invalid_assn_def
+          pred_lift_extract_simps)
+    done
+  show ?thesis
+    supply [vcg_rules] = cl_fold_monadic'_nres_rule[where A=A and B=B and fi=fi and f=f, OF BODY]
+    by (sepref_to_hoare; vcg)
+qed
+
+definition cl_ifoldl_guard
+  :: \<open>'a::llvm_rep \<times> 'b::llvm_rep cl_list \<times> 'c::llvm_rep cl_list \<times> 1 word \<Rightarrow> 1 word llM\<close>
+  where [llvm_code, llvm_inline]:
+  \<open>cl_ifoldl_guard \<equiv> \<lambda>(acc, xp, yp, stop). doM {
+      if to_bool stop then Mreturn 0
+      else if xp = null then Mreturn 0
+      else if yp = null then Mreturn 0
+      else Mreturn 1}\<close>
+
+definition cl_ifoldl ::
+  \<open>('a::llvm_rep \<Rightarrow> 'b::llvm_rep \<Rightarrow> 'c::llvm_rep \<Rightarrow> 8 word \<Rightarrow> 'a llM)
+    \<Rightarrow> ('b \<Rightarrow> 'c \<Rightarrow> 8 word llM)
+    \<Rightarrow> ('a \<Rightarrow> 'b \<Rightarrow> 'a llM) \<Rightarrow> ('a \<Rightarrow> 'c \<Rightarrow> 'a llM)
+    \<Rightarrow> 'a \<Rightarrow> 'b cl_list \<Rightarrow> 'c cl_list \<Rightarrow> 'a llM\<close>
+  where [llvm_code]:
+  \<open>cl_ifoldl f dec f1 f2 acc xp yp \<equiv> doM {
+    (acc, xp, yp, stop) \<leftarrow> llc_while cl_ifoldl_guard
+    (\<lambda>(acc, xp, yp, stop). doM {
+      xn \<leftarrow> ll_load xp;
+      yn \<leftarrow> ll_load yp;
+      let x = node.val xn;
+      let y = node.val yn;
+      dir \<leftarrow> dec x y;
+      acc \<leftarrow> f acc x y dir;
+      if dir = 0 then
+        Mreturn (acc, node.next xn, node.next yn, 1)
+      else if dir = 1 then
+        Mreturn (acc, node.next xn, yp, 0)
+      else if dir = 2 then
+        Mreturn (acc, xp, node.next yn, 0)
+      else
+        Mreturn (acc, node.next xn, node.next yn, 0)
+    }) (acc, xp, yp, 0 :: 1 word);
+    if to_bool stop then
+      Mreturn acc
+    else if yp = null then
+      cl_foldl_monadic' f1 (acc, xp)
+    else if xp = null then
+      cl_foldl_monadic' f2 (acc, yp)
+    else
+      Mreturn acc
+  }\<close>
+
+subsection \<open>Direction encoding\<close>
+
+definition dir_enc :: \<open>direction \<Rightarrow> 8 word\<close> where
+  \<open>dir_enc d \<equiv> case d of STOP \<Rightarrow> 0 | LEFT \<Rightarrow> 1 | RIGHT \<Rightarrow> 2 | BOTH \<Rightarrow> 3\<close>
+
+lemma dir_enc_simps[simp]:
+  \<open>dir_enc STOP = 0\<close> \<open>dir_enc LEFT = 1\<close> \<open>dir_enc RIGHT = 2\<close> \<open>dir_enc BOTH = 3\<close>
+  by (simp_all add: dir_enc_def)
+
+lemma dir_enc_eq_iff[simp]:
+  \<open>dir_enc d = 0 \<longleftrightarrow> d = STOP\<close>
+  \<open>dir_enc d = 1 \<longleftrightarrow> d = LEFT\<close>
+  \<open>dir_enc d = 2 \<longleftrightarrow> d = RIGHT\<close>
+  \<open>dir_enc d = 3 \<longleftrightarrow> d = BOTH\<close>
+  by (cases d; simp)+
+
+definition dir_rel :: \<open>(8 word \<times> direction) set\<close> where
+  \<open>dir_rel \<equiv> {(w, d). w = dir_enc d}\<close>
+
+definition dir_assn :: \<open>direction \<Rightarrow> 8 word \<Rightarrow> assn\<close> where
+  \<open>dir_assn \<equiv> pure dir_rel\<close>
+
+lemma dir_assn_simp[simp]: \<open>dir_assn d w = \<up>(w = dir_enc d)\<close>
+  unfolding dir_assn_def dir_rel_def by (simp add: pure_app_eq)
+
+context begin
+interpretation llvm_prim_arith_setup .
+
+lemma ll_ptrcmp_eq_null_simp:
+  \<open>ll_ptrcmp_eq a null = doM { Mreturn (from_bool (a = null))}\<close>
+  by (vcg_normalize; simp add: eq_commute[of null])
+
+lemma ll_ptrcmp_eq_null_rule[vcg_rules]:
+  \<open>llvm_htriple \<box> (ll_ptrcmp_eq a null) (\<lambda>r. \<up>(to_bool r \<longleftrightarrow> a = null))\<close>
+  unfolding ll_ptrcmp_eq_null_simp
+  by vcg
+
+lemma ll_icmp_eq_bool_rule:
+  \<open>llvm_htriple \<box> (ll_icmp_eq (a::'l::len word) b) (\<lambda>r. \<up>(to_bool r \<longleftrightarrow> a = b))\<close>
+  by vcg
+
+end
+
+subsection \<open>Hoare rule for @{term cl_ifoldl}\<close>
+lemma cl_ifoldl_guard_rule[vcg_rules]:
+  \<open>llvm_htriple \<box> (cl_ifoldl_guard (acci, xp, yp, stop))
+    (\<lambda>r. \<upharpoonleft>bool.assn (stop = 0 \<and> xp \<noteq> null \<and> yp \<noteq> null) r)\<close>
+proof -
+  interpret llvm_prim_ctrl_setup .
+  show ?thesis
+    unfolding cl_ifoldl_guard_def
+    supply [simp] = bool.assn_def
+    by vcg
+qed
+
+lemma cl_assn'_load_rule:
+  \<open>llvm_htriple (cl_assn' A xs p ** \<up>(p \<noteq> null)) (ll_load p)
+    (\<lambda>r. EXS c q. \<up>(r = Node c q \<and> xs \<noteq> []) ** \<upharpoonleft>ll_bpto (Node c q) p
+        ** A (hd xs) c ** cl_assn' A (tl xs) q)\<close>
+proof (cases xs)
+  case Nil
+  then show ?thesis by (simp add: cl_assn_simps) vcg
+next
+  case (Cons x xs')
+  then show ?thesis by (simp add: cl_assn_simps) vcg
+qed
+
+lemma olseg_snoc_red:
+  \<open>PRECOND (SOLVE_AUTO (i < length xs)) \<Longrightarrow>
+    is_sep_red \<box> (\<upharpoonleft>ll_bpto (Node c r) q ** A (xs ! i) c)
+      (olseg A (take i xs) p q) (olseg A (take (Suc i) xs) p r)\<close>
+  unfolding vcg_tag_defs
+proof (rule is_sep_redI)
+  fix Ps Qs
+  assume I: \<open>i < length xs\<close>
+    and H: \<open>\<box> ** Ps \<turnstile> (\<upharpoonleft>ll_bpto (Node c r) q ** A (xs ! i) c) ** Qs\<close>
+  have H': \<open>Ps \<turnstile> \<upharpoonleft>ll_bpto (Node c r) q ** A (xs ! i) c ** Qs\<close>
+    using H by simp
+  have 1: \<open>olseg A (take i xs) p q ** Ps
+      \<turnstile> (olseg A (take i xs) p q ** \<upharpoonleft>ll_bpto (Node c r) q ** A (xs ! i) c) ** Qs\<close>
+    using conj_entails_mono[OF entails_refl H'] unfolding sep_conj_assoc .
+  have 2: \<open>(olseg A (take i xs) p q ** \<upharpoonleft>ll_bpto (Node c r) q ** A (xs ! i) c) ** Qs
+      \<turnstile> olseg A (take (Suc i) xs) p r ** Qs\<close>
+    using conj_entails_mono[OF olseg_snoc entails_refl, of A \<open>take i xs\<close> p q c r \<open>xs ! i\<close> Qs]
+    by (simp add: take_Suc_conv_app_nth[OF I])
+  show \<open>olseg A (take i xs) p q ** Ps \<turnstile> olseg A (take (Suc i) xs) p r ** Qs\<close>
+    by (rule entails_trans[OF 1 2])
+qed
+
+lemma olseg_cl_reassemble_red:
+  \<open>is_sep_red \<box> (cl_assn' A (drop i xs) q) (olseg A (take i xs) p q) (cl_assn' A xs p)\<close>
+proof (rule is_sep_redI)
+  fix Ps Qs
+  assume H: \<open>\<box> ** Ps \<turnstile> cl_assn' A (drop i xs) q ** Qs\<close>
+  have H': \<open>Ps \<turnstile> olseg A (drop i xs) q null ** Qs\<close>
+    using H by (simp add: cl_assn_olseg)
+  have 1: \<open>olseg A (take i xs) p q ** Ps
+      \<turnstile> (olseg A (take i xs) p q ** olseg A (drop i xs) q null) ** Qs\<close>
+    using conj_entails_mono[OF entails_refl H'] unfolding sep_conj_assoc .
+  have 2: \<open>(olseg A (take i xs) p q ** olseg A (drop i xs) q null) ** Qs
+      \<turnstile> cl_assn' A xs p ** Qs\<close>
+    using conj_entails_mono[OF olseg_append entails_refl, of A \<open>take i xs\<close> p q \<open>drop i xs\<close> null Qs]
+    by (simp add: cl_assn_olseg)
+  show \<open>olseg A (take i xs) p q ** Ps \<turnstile> cl_assn' A xs p ** Qs\<close>
+    by (rule entails_trans[OF 1 2])
+qed
+
+lemma cl_assn'_cons_red:
+  \<open>PRECOND (SOLVE_AUTO (i < length xs)) \<Longrightarrow>
+    is_sep_red \<box> (A (xs ! i) c ** cl_assn' A (drop (Suc i) xs) q)
+      (\<upharpoonleft>ll_bpto (Node c q) p) (cl_assn' A (drop i xs) p)\<close>
+  unfolding vcg_tag_defs
+proof (rule is_sep_redI)
+  fix Ps Qs
+  assume I: \<open>i < length xs\<close>
+    and H: \<open>\<box> ** Ps \<turnstile> (A (xs ! i) c ** cl_assn' A (drop (Suc i) xs) q) ** Qs\<close>
+  have H': \<open>Ps \<turnstile> A (xs ! i) c ** cl_assn' A (drop (Suc i) xs) q ** Qs\<close>
+    using H by simp
+  have E: \<open>cl_assn' A (drop i xs) p
+      = (EXS c q. \<upharpoonleft>ll_bpto (Node c q) p ** A (xs ! i) c ** cl_assn' A (drop (Suc i) xs) q)\<close>
+    by (subst Cons_nth_drop_Suc[OF I, symmetric]) (simp add: cl_assn_simps)
+  have 1: \<open>\<upharpoonleft>ll_bpto (Node c q) p ** Ps
+      \<turnstile> (\<upharpoonleft>ll_bpto (Node c q) p ** A (xs ! i) c ** cl_assn' A (drop (Suc i) xs) q) ** Qs\<close>
+    using conj_entails_mono[OF entails_refl H'] unfolding sep_conj_assoc .
+  have 2: \<open>\<upharpoonleft>ll_bpto (Node c q) p ** A (xs ! i) c ** cl_assn' A (drop (Suc i) xs) q
+      \<turnstile> cl_assn' A (drop i xs) p\<close>
+    unfolding E
+    by (rule entails_exI[where x=c], rule entails_exI[where x=q], rule entails_refl)
+  show \<open>\<upharpoonleft>ll_bpto (Node c q) p ** Ps \<turnstile> cl_assn' A (drop i xs) p ** Qs\<close>
+    by (rule entails_trans[OF 1 conj_entails_mono[OF 2 entails_refl]])
+qed
+
+context begin
+
+private lemma cl_assn'_cong_fri:
+  \<open>PRECOND (SOLVE_AUTO (a = a')) \<Longrightarrow> cl_assn' A a c \<turnstile> cl_assn' A a' c\<close>
+  unfolding vcg_tag_defs by simp
+
+private lemma olseg_empty_fri:
+  \<open>PRECOND (SOLVE_AUTO (ys = [] \<and> p = q)) \<Longrightarrow> \<box> \<turnstile> olseg A ys p q\<close>
+  unfolding vcg_tag_defs by (simp add: olseg_nil sep_algebra_simps)
+
+private lemma olseg_cl_fri:
+  \<open>PRECOND (SOLVE_AUTO (ys = xs)) \<Longrightarrow> olseg A ys p null \<turnstile> cl_assn' A xs p\<close>
+  unfolding vcg_tag_defs by (simp add: cl_assn_olseg)
+
+private lemma drop_head:
+  \<open>i < length xs \<Longrightarrow> drop i xs = xs ! i # drop (Suc i) xs\<close>
+  by (simp add: Cons_nth_drop_Suc)
+
+lemma cl_ifoldl_rule:
+  assumes F: \<open>\<And>a ai b bi c ci d di. llvm_htriple
+    (A a ai ** B b bi ** C c ci ** dir_assn d di)
+    (fi ai bi ci di)
+    (\<lambda>r. A (f a b c d) r ** B b bi ** C c ci)\<close>
+    and DEC: \<open>\<And>b bi c ci. llvm_htriple
+    (B b bi ** C c ci)
+    (deci bi ci)
+    (\<lambda>r. dir_assn (dec b c) r ** B b bi ** C c ci)\<close>
+    and F1: \<open>\<And>a ai b bi. llvm_htriple
+    (A a ai ** B b bi)
+    (f1i ai bi)
+    (\<lambda>r. A (f1 a b) r ** B b bi)\<close>
+    and F2: \<open>\<And>a ai c ci. llvm_htriple
+    (A a ai ** C c ci)
+    (f2i ai ci)
+    (\<lambda>r. A (f2 a c) r ** C c ci)\<close>
+  shows \<open>llvm_htriple
+    (A acc acci ** cl_assn' B bs bsi ** cl_assn' C cs csi)
+    (cl_ifoldl fi deci f1i f2i acci bsi csi)
+    (\<lambda>r. A (ifoldl f dec f1 f2 acc bs cs) r ** cl_assn' B bs bsi ** cl_assn' C cs csi)\<close>
+proof -
+  interpret llvm_prim_ctrl_setup .
+  show ?thesis
+  unfolding cl_ifoldl_def
+  apply (rewrite annotate_llc_while [where
+    I = \<open>\<lambda>(acci', xp, yp, stop) t. EXS i j acc'.
+        A acc' acci'
+        ** olseg B (take i bs) bsi xp ** olseg C (take j cs) csi yp
+        ** cl_assn' B (drop i bs) xp ** cl_assn' C (drop j cs) yp
+        ** \<up>((if stop = 0
+               then ifoldl f dec f1 f2 acc' (drop i bs) (drop j cs)
+               else acc')
+              = ifoldl f dec f1 f2 acc bs cs)
+        ** \<up>\<^sub>!(t = (if stop = 0 then Suc (length bs - i + (length cs - j)) else 0))\<close>
+    and R = \<open>measure id\<close>])
+  supply [vcg_rules] = F DEC ll_icmp_eq_bool_rule cl_assn'_load_rule
+    cl_fold_monadic'_rule[where A=A and B=B and fi=f1i and f=f1, OF F1]
+    cl_fold_monadic'_rule[where A=A and B=C and fi=f2i and f=f2, OF F2]
+  supply [simp] = cl_assn_simps olseg_nil sep_conj_exists drop_head
+    hd_drop_conv_nth drop_Suc[symmetric] ifoldl_Nil1 ifoldl_Nil2
+  supply [fri_rules] = cl_assn'_cong_fri olseg_empty_fri olseg_cl_fri
+  supply [fri_red_rules] = olseg_snoc_red olseg_cl_reassemble_red cl_assn'_cons_red
+  apply vcg_monadify
+  apply vcg'
+  subgoal for aa ab x xa
+    by (cases \<open>dec (bs ! x) (cs ! xa)\<close>) auto
+  done
+qed
+
+
+subsection \<open>Refinement rule for @{term cl_ifoldl} against @{term ifoldl_nres}\<close>
+lemma cl_ifoldl_nres_rule:
+  assumes F: \<open>\<And>a ai b bi c ci d di. nofail (fn a b c d) \<Longrightarrow> llvm_htriple
+    (A a ai ** B b bi ** C c ci ** dir_assn d di)
+    (fi ai bi ci di)
+    (\<lambda>r. B b bi ** C c ci ** (EXS x. A x r ** \<up>(RETURN x \<le> fn a b c d)))\<close>
+    and DEC: \<open>\<And>b bi c ci. nofail (decn b c) \<Longrightarrow> llvm_htriple
+    (B b bi ** C c ci)
+    (deci bi ci)
+    (\<lambda>r. B b bi ** C c ci ** (EXS d. dir_assn d r ** \<up>(RETURN d \<le> decn b c)))\<close>
+    and F1: \<open>\<And>a ai b bi. nofail (f1n a b) \<Longrightarrow> llvm_htriple
+    (A a ai ** B b bi)
+    (f1i ai bi)
+    (\<lambda>r. B b bi ** (EXS x. A x r ** \<up>(RETURN x \<le> f1n a b)))\<close>
+    and F2: \<open>\<And>a ai c ci. nofail (f2n a c) \<Longrightarrow> llvm_htriple
+    (A a ai ** C c ci)
+    (f2i ai ci)
+    (\<lambda>r. C c ci ** (EXS x. A x r ** \<up>(RETURN x \<le> f2n a c)))\<close>
+    and NF: \<open>nofail (ifoldl_nres fn decn f1n f2n acc bs cs)\<close>
+  shows \<open>llvm_htriple
+    (A acc acci ** cl_assn' B bs bsi ** cl_assn' C cs csi)
+    (cl_ifoldl fi deci f1i f2i acci bsi csi)
+    (\<lambda>r. cl_assn' B bs bsi ** cl_assn' C cs csi
+      ** (EXS x. A x r ** \<up>(RETURN x \<le> ifoldl_nres fn decn f1n f2n acc bs cs)))\<close>
+proof -
+  interpret llvm_prim_ctrl_setup .
+  show ?thesis
+  using NF
+  unfolding cl_ifoldl_def
+  apply (rewrite annotate_llc_while [where
+    I = \<open>\<lambda>(acci', xp, yp, stop) t. EXS i j acc'.
+        A acc' acci'
+        ** olseg B (take i bs) bsi xp ** olseg C (take j cs) csi yp
+        ** cl_assn' B (drop i bs) xp ** cl_assn' C (drop j cs) yp
+        ** \<up>((if stop = 0
+               then ifoldl_nres fn decn f1n f2n acc' (drop i bs) (drop j cs)
+               else RETURN acc')
+              \<le> ifoldl_nres fn decn f1n f2n acc bs cs)
+        ** \<up>\<^sub>!(t = (if stop = 0 then Suc (length bs - i + (length cs - j)) else 0))\<close>
+    and R = \<open>measure id\<close>])
+  supply [vcg_rules] = F DEC ll_icmp_eq_bool_rule cl_assn'_load_rule
+    cl_fold_monadic'_nres_rule'[where A=A and B=B and fi=f1i and f=f1n, OF F1]
+    cl_fold_monadic'_nres_rule'[where A=A and B=C and fi=f2i and f=f2n, OF F2]
+  supply [simp] = cl_assn_simps olseg_nil sep_conj_exists drop_head
+    hd_drop_conv_nth drop_Suc[symmetric] ifoldl_nres_Nil1 ifoldl_nres_Nil2 ifoldl_nres_Cons
+    pw_le_iff refine_pw_simps
+  supply [fri_rules] = cl_assn'_cong_fri olseg_empty_fri olseg_cl_fri
+  supply [fri_red_rules] = olseg_snoc_red olseg_cl_reassemble_red cl_assn'_cons_red
+  apply vcg_monadify
+  apply vcg'
+  apply (auto split: direction.splits)
+  subgoal by blast
+  subgoal by blast
+  subgoal by blast
+  subgoal by (meson direction.exhaust)
+  subgoal by metis
+  done
+qed
+
+end
+
+subsection \<open>hfref forms\<close>
+
+lemma hfref_nres_htriple_d1_k2_k3_k4:
+  assumes R: \<open>(uncurry3 fi, uncurry3 fn) \<in> A\<^sup>d *\<^sub>a B\<^sup>k *\<^sub>a C\<^sup>k *\<^sub>a dir_assn\<^sup>k \<rightarrow>\<^sub>a A\<close>
+    and NF: \<open>nofail (fn a b c d)\<close>
+  shows \<open>llvm_htriple (A a ai ** B b bi ** C c ci ** dir_assn d di) (fi ai bi ci di)
+    (\<lambda>r. B b bi ** C c ci ** (EXS x. A x r ** \<up>(RETURN x \<le> fn a b c d)))\<close>
+proof -
+  note HT = R[to_hnr, unfolded autoref_tag_defs, THEN hn_refineD, OF NF]
+  show ?thesis
+    apply (rule htriple_ent_pre[OF _ htriple_ent_post[OF _ HT]])
+    unfolding hn_ctxt_def
+    subgoal by (rule entails_refl)
+    subgoal
+      by (auto simp: entails_def sep_algebra_simps sep_conj_exists invalid_assn_def
+          pred_lift_extract_simps)
+    done
+qed
+
+lemma hfref_nres_htriple_k1_k2:
+  assumes R: \<open>(uncurry fi, uncurry fn) \<in> B\<^sup>k *\<^sub>a C\<^sup>k \<rightarrow>\<^sub>a D\<close>
+    and NF: \<open>nofail (fn b c)\<close>
+  shows \<open>llvm_htriple (B b bi ** C c ci) (fi bi ci)
+    (\<lambda>r. B b bi ** C c ci ** (EXS x. D x r ** \<up>(RETURN x \<le> fn b c)))\<close>
+proof -
+  note HT = R[to_hnr, unfolded autoref_tag_defs, THEN hn_refineD, OF NF]
+  show ?thesis
+    apply (rule htriple_ent_pre[OF _ htriple_ent_post[OF _ HT]])
+    unfolding hn_ctxt_def
+    subgoal by (rule entails_refl)
+    subgoal
+      by (auto simp: entails_def sep_algebra_simps sep_conj_exists
+          pred_lift_extract_simps)
+    done
+qed
+
+lemma hfref_nres_htriple_d1_k2:
+  assumes R: \<open>(uncurry fi, uncurry fn) \<in> A\<^sup>d *\<^sub>a B\<^sup>k \<rightarrow>\<^sub>a A\<close>
+    and NF: \<open>nofail (fn a b)\<close>
+  shows \<open>llvm_htriple (A a ai ** B b bi) (fi ai bi)
+    (\<lambda>r. B b bi ** (EXS x. A x r ** \<up>(RETURN x \<le> fn a b)))\<close>
+proof -
+  note HT = R[to_hnr, unfolded autoref_tag_defs, THEN hn_refineD, OF NF]
+  show ?thesis
+    apply (rule htriple_ent_pre[OF _ htriple_ent_post[OF _ HT]])
+    unfolding hn_ctxt_def
+    subgoal by (rule entails_refl)
+    subgoal
+      by (auto simp: entails_def sep_algebra_simps sep_conj_exists invalid_assn_def
+          pred_lift_extract_simps)
+    done
+qed
+
+lemma cl_ifoldl_nres_hfref:
+  assumes F: \<open>(uncurry3 fi, uncurry3 fn) \<in> A\<^sup>d *\<^sub>a B\<^sup>k *\<^sub>a C\<^sup>k *\<^sub>a dir_assn\<^sup>k \<rightarrow>\<^sub>a A\<close>
+    and DEC: \<open>(uncurry deci, uncurry decn) \<in> B\<^sup>k *\<^sub>a C\<^sup>k \<rightarrow>\<^sub>a dir_assn\<close>
+    and F1: \<open>(uncurry f1i, uncurry f1n) \<in> A\<^sup>d *\<^sub>a B\<^sup>k \<rightarrow>\<^sub>a A\<close>
+    and F2: \<open>(uncurry f2i, uncurry f2n) \<in> A\<^sup>d *\<^sub>a C\<^sup>k \<rightarrow>\<^sub>a A\<close>
+  shows \<open>(uncurry2 (cl_ifoldl fi deci f1i f2i), uncurry2 (ifoldl_nres fn decn f1n f2n))
+    \<in> A\<^sup>d *\<^sub>a (cl_assn' B)\<^sup>k *\<^sub>a (cl_assn' C)\<^sup>k \<rightarrow>\<^sub>a A\<close>
+  supply [vcg_rules] = cl_ifoldl_nres_rule[where A=A and B=B and C=C
+      and fi=fi and deci=deci and f1i=f1i and f2i=f2i
+      and fn=fn and decn=decn and f1n=f1n and f2n=f2n,
+      OF hfref_nres_htriple_d1_k2_k3_k4[OF F] hfref_nres_htriple_k1_k2[OF DEC]
+         hfref_nres_htriple_d1_k2[OF F1] hfref_nres_htriple_d1_k2[OF F2]]
+  by (sepref_to_hoare; vcg)
+
+text \<open>The functional variant follows by monotonicity of \<open>hfref\<close> in the
+  abstract program, via @{thm ifoldl_nres_refine}.\<close>
+lemma cl_ifoldl_hfref:
+  assumes F: \<open>(uncurry3 fi, uncurry3 (RETURN oooo f))
+      \<in> A\<^sup>d *\<^sub>a B\<^sup>k *\<^sub>a C\<^sup>k *\<^sub>a dir_assn\<^sup>k \<rightarrow>\<^sub>a A\<close>
+    and DEC: \<open>(uncurry deci, uncurry (RETURN oo dec)) \<in> B\<^sup>k *\<^sub>a C\<^sup>k \<rightarrow>\<^sub>a dir_assn\<close>
+    and F1: \<open>(uncurry f1i, uncurry (RETURN oo f1)) \<in> A\<^sup>d *\<^sub>a B\<^sup>k \<rightarrow>\<^sub>a A\<close>
+    and F2: \<open>(uncurry f2i, uncurry (RETURN oo f2)) \<in> A\<^sup>d *\<^sub>a C\<^sup>k \<rightarrow>\<^sub>a A\<close>
+  shows \<open>(uncurry2 (cl_ifoldl fi deci f1i f2i), uncurry2 (RETURN ooo ifoldl f dec f1 f2))
+    \<in> A\<^sup>d *\<^sub>a (cl_assn' B)\<^sup>k *\<^sub>a (cl_assn' C)\<^sup>k \<rightarrow>\<^sub>a A\<close>
+proof -
+  note M = cl_ifoldl_nres_hfref[OF F DEC F1 F2]
+  have LE: \<open>ifoldl_nres (RETURN oooo f) (RETURN oo dec) (RETURN oo f1) (RETURN oo f2)
+      acc bs cs \<le> RETURN (ifoldl f dec f1 f2 acc bs cs)\<close> for acc bs cs
+    by (rule order_trans[OF ifoldl_nres_refine]) (simp_all add: pw_le_iff refine_pw_simps)
+  show ?thesis
+    apply (rule hfrefI)
+    apply (rule hn_refine_ref[OF _ hfrefD[OF M]])
+    by (auto simp: LE)
+qed
+
+subsection \<open>Sepref setup for @{typ direction}\<close>
+
+lemma dir_enc_inj[simp]: \<open>dir_enc d = dir_enc d' \<longleftrightarrow> d = d'\<close>
+  by (cases d; cases d'; simp)
+
+lemma dir_assn_is_pure[safe_constraint_rules]: \<open>is_pure dir_assn\<close>
+  unfolding dir_assn_def by simp
+
+lemma dir_assn_free[sepref_frame_free_rules]: \<open>MK_FREE dir_assn (\<lambda>_. Mreturn ())\<close>
+  unfolding dir_assn_def by (rule mk_free_pure)
+
+sepref_register STOP LEFT RIGHT BOTH
+sepref_register eq_dir: \<open>(=) :: direction \<Rightarrow> _\<close> :: \<open>direction \<Rightarrow> direction \<Rightarrow> bool\<close>
+
+lemma dir_const_hnr[sepref_fr_rules]:
+  \<open>(uncurry0 (Mreturn (0 :: 8 word)), uncurry0 (RETURN STOP)) \<in> unit_assn\<^sup>k \<rightarrow>\<^sub>a dir_assn\<close>
+  \<open>(uncurry0 (Mreturn (1 :: 8 word)), uncurry0 (RETURN LEFT)) \<in> unit_assn\<^sup>k \<rightarrow>\<^sub>a dir_assn\<close>
+  \<open>(uncurry0 (Mreturn (2 :: 8 word)), uncurry0 (RETURN RIGHT)) \<in> unit_assn\<^sup>k \<rightarrow>\<^sub>a dir_assn\<close>
+  \<open>(uncurry0 (Mreturn (3 :: 8 word)), uncurry0 (RETURN BOTH)) \<in> unit_assn\<^sup>k \<rightarrow>\<^sub>a dir_assn\<close>
+  by (sepref_to_hoare; vcg)+
+
+lemma dir_eq_hnr[sepref_fr_rules]:
+  \<open>(uncurry ll_icmp_eq, uncurry (RETURN oo (=))) \<in> dir_assn\<^sup>k *\<^sub>a dir_assn\<^sup>k \<rightarrow>\<^sub>a bool1_assn\<close>
+  supply [vcg_rules] = ll_icmp_eq_bool_rule
+  supply [simp] = pure_def bool1_rel_def bool.rel_def in_br_conv
+  by (sepref_to_hoare; vcg)
+
+experiment
+begin
+
+text \<open>Non-monadic test refinement\<close>
+abbreviation \<open>u8_assn \<equiv> unat_assn' TYPE(8)\<close>
+definition \<open>ftest a b c dir \<equiv>
+  if dir = STOP then a
+  else if dir = LEFT then c # b # a
+  else if dir = RIGHT then b # c # a
+  else b # a
+\<close>
+sepref_def ftest_impl is \<open>uncurry3 (RETURN oooo ftest)\<close>
+  :: \<open>(cl_assn' u8_assn)\<^sup>d *\<^sub>a u8_assn\<^sup>k *\<^sub>a u8_assn\<^sup>k *\<^sub>a dir_assn\<^sup>k \<rightarrow>\<^sub>a (cl_assn' u8_assn)\<close>
+  unfolding ftest_def
+  by sepref
+
+definition \<open>dirtest a b \<equiv>
+  if a = b then BOTH
+  else if a < b then LEFT
+  else RIGHT
+\<close>
+sepref_def dirtest_impl is \<open>uncurry (RETURN oo dirtest)\<close>
+  :: \<open>u8_assn\<^sup>k *\<^sub>a u8_assn\<^sup>k \<rightarrow>\<^sub>a dir_assn\<close>
+  unfolding dirtest_def
+  by sepref
+
+definition \<open>f1test a b = b # a\<close>
+sepref_def f1test_impl is \<open>uncurry (RETURN oo f1test)\<close>
+  :: \<open>(cl_assn' u8_assn)\<^sup>d *\<^sub>a u8_assn\<^sup>k \<rightarrow>\<^sub>a cl_assn' u8_assn\<close>
+  unfolding f1test_def
+  by sepref
+
+definition \<open>f2test a c = c # a\<close>
+sepref_def f2test_impl is \<open>uncurry (RETURN oo f2test)\<close>
+  :: \<open>(cl_assn' u8_assn)\<^sup>d *\<^sub>a u8_assn\<^sup>k \<rightarrow>\<^sub>a cl_assn' u8_assn\<close>
+  unfolding f2test_def
+  by sepref
+
+definition \<open>test_ifoldl \<equiv> ifoldl ftest dirtest f1test f2test\<close>
+sepref_register test_ifoldl
+
+lemmas test_ifoldl_hnr[sepref_fr_rules] =
+  cl_ifoldl_hfref[OF ftest_impl.refine dirtest_impl.refine f1test_impl.refine f2test_impl.refine,
+    folded test_ifoldl_def]
+
+definition \<open>test \<equiv> ifoldl ftest dirtest f1test f2test []\<close>
+
+sepref_def test_impl is \<open>uncurry (RETURN oo test)\<close>
+  :: \<open>(cl_assn' u8_assn)\<^sup>k *\<^sub>a (cl_assn' u8_assn)\<^sup>k \<rightarrow>\<^sub>a cl_assn' u8_assn\<close>
+  unfolding test_def test_ifoldl_def[symmetric]
+  by sepref
+
+end
 
 end
